{
 "cells": [
  {
   "attachments": {},
   "cell_type": "markdown",
   "metadata": {},
   "source": [
    "$ 2. Efetue:$\n",
    "\n",
    "$a) (3+j2)+(2-j5)$\n",
    "$$\n",
    "\\begin{align*}\n",
    "(3+j2)+(2-j5) &= (3+2)+j(2-5)\\\\ &=5-j3\n",
    "\\end{align*}\n",
    "$$\n",
    "\n",
    "$b) (5-j2)-(2-j8)$\n",
    "$$\n",
    "\\begin{align*}\n",
    " (5-j2)-(2-j8) &= (5-2)+j(8-2)\\\\ &= 3+j6\n",
    "\\end{align*}\n",
    "$$b\n",
    "\n",
    "$c) (1+j)+(1-j)-j2$\n",
    "$$\n",
    "\\begin{align*}\n",
    " (1+1)+j-j-j2 &=\\\\ 1+1-j2 &=2-j2\n",
    "\\end{align*}\n",
    "$$\n",
    "\n",
    "$d) (6+j7)-(4+j2)-(1-j10)$\n",
    "$$\n",
    "\\begin{align*}\n",
    " (6-4+1)+j(7-2-10)&= 3-j5\n",
    "\\end{align*}\n",
    "$$\n"
   ]
  },
  {
   "attachments": {},
   "cell_type": "markdown",
   "metadata": {},
   "source": [
    "$ 3. Efetue:$\n",
    "$a) (2-j3)(1+j5)$\n",
    "$$\n",
    "\\begin{align*}\n",
    "2\\cdot 1 +2\\cdot j5 -j3\\cdot 1 -3\\cdot 5 j^2 &= 2+j10-j3+15 \\\\ (2-j3)(1+j5) = 17+j7\n",
    "\\end{align*}\n",
    "$$\n",
    "\n",
    "$b) (1+j2)(2+j)$\n",
    "$$\n",
    "\\begin{align*}\n",
    "1 \\cdot 2 + j + 2\\cdot j2 +2j^2 &= 2 + j + j5 -2 \\\\ (1+j2)(2+j)&=j5\n",
    "\\end{align*}\n",
    "$$\n",
    "\n",
    "$c) (4-j3)(5-j)(1+j)$\n",
    "$$\n",
    "\\begin{align*}\n",
    "(4\\cdot 5-j4-3\\cdot 5j+3j^2)(1+j)\\\\\n",
    "(20-j4-j15-3)(1+j)&=(17-j19)(1+j)\\\\ 17+j17-j19-19j^2 &= 36-j2\n",
    "\\end{align*}\n",
    "$$\n",
    "\n",
    "$d)(7+j2)(7-j2)$\n",
    "$$\n",
    "\\begin{align*}\n",
    "7\\cdot 7 -j2\\cdot 7+j2\\cdot 7-2\\cdot 2 j^2 &=49-4j^2 \\\\ (7+j2)(7-j2)&=45\n",
    "\n",
    "\\end{align*}\n",
    "$$"
   ]
  },
  {
   "attachments": {},
   "cell_type": "markdown",
   "metadata": {},
   "source": [
    "$4.\\ Se \\ u= 4+j3 e v = 5-j2, calcule \\ u\\cdot v.$\n",
    "$$\n",
    "\\begin{align*}\n",
    "u\\cdot v &= (4+j3)(5-j2)\\\\ u\\cdot v &= 4\\cdot 5-4\\cdot j2+j3\\cdot 5-2\\cdot 3j^2 \\\\u\\cdot v &= 20 -j8+j15-6j^2\\\\u\\cdot v &= 26+j6\n",
    "\\end{align*}\n",
    "$$"
   ]
  },
  {
   "attachments": {},
   "cell_type": "markdown",
   "metadata": {},
   "source": [
    "$ 5. Calcule:\\\\$\n",
    "$a) (3+j2)^2$\n",
    "$$\n",
    "\\begin{align*}\n",
    "(3+j2)^2 &=3^2+2\\cdot 3\\cdot j2 +(j2)^2\\\\(3+j2)^2 &= 9+j12+4j^2\\\\ (3+j2)^2 &= 5+j12\n",
    "\\end{align*}\n",
    "$$\n",
    "\n",
    "$b) (5-j)^2$\n",
    "$$\n",
    "\\begin{align*}\n",
    "(5-j)^2&= 5^2-2\\cdot 5\\cdot j +j^2 \\\\ (5-j)^2&= 25-j10-1 \\\\(5-j)^2&=24-j10\n",
    "\\end{align*}\n",
    "$$\n",
    "\n",
    "$c) (1+j)^2$\n",
    "$$\n",
    "\\begin{align*}\n",
    "(1+j)^2&= 1^2+2\\cdot 1\\cdot j +j^2 \\\\ (1+j)^2&= 1+j2-1\\\\(1+j)^2&=j2\n",
    "\\end{align*}\n",
    "$$\n"
   ]
  },
  {
   "attachments": {},
   "cell_type": "markdown",
   "metadata": {},
   "source": [
    "$6. \\ Se\\ f(z) = z^2-z+1,\\ calcule f(1-j).$\n",
    "$$\n",
    "\\begin{align*}\n",
    "f(1-j) &= (1-j)^2-(1-j)+1 \\\\ f(1-j) &=1-j2+j^2-1+j+1\\\\f(1-j) &=-j2\n",
    "\\end{align*}\n",
    "$$"
   ]
  },
  {
   "attachments": {},
   "cell_type": "markdown",
   "metadata": {},
   "source": [
    "$7.\\ f(z)= z^4+jz^3-(1+j2)z^2 + 3z+1+j3, \\ calcule f(1+j).$\n",
    "$$\n",
    "\\begin{align*}\n",
    "f(1+j)&= (1+j)^4 - j(1+j)^3 -(1+j2)(1+j)^2+3(1+j)+1+j3\\\\\n",
    "f(1+j)&=j2\\cdot j2 -j(j2\\cdot (1+j))-(1+j2)\\cdot j2+3+j3+1+j3 \\\\\n",
    "f(1+j)+&= 4j^2-j(j2+2j^2)-(j2+4j^2)+4+j6\\\\ \n",
    "f(1+j)&= -j(j2-2)-(j2-4)+j6\\\\\n",
    "f(1+j)&= 2j^2-j2-j2+4+j6\\\\\n",
    "f(1+j)&= 2+j2\n",
    "\\end{align*}\n",
    "$$"
   ]
  },
  {
   "cell_type": "code",
   "execution_count": 1,
   "metadata": {},
   "outputs": [
    {
     "name": "stdout",
     "output_type": "stream",
     "text": [
      "(2+2j)\n"
     ]
    }
   ],
   "source": [
    "z = (1+1j)\n",
    "print(z**4+1j*z**3-(1+2j)*z**2+3*z+1+3J)"
   ]
  },
  {
   "attachments": {},
   "cell_type": "markdown",
   "metadata": {},
   "source": [
    "$8.\\ Prove\\ que\\ (1+j)^2 =j2\\ e \\ coloque\\ na\\ forma\\ algebrica\\ o\\ numero\\ \\\\ z = \\frac{(1+j)^80-(1+j)^82}{j^96}$\n",
    "$$\n",
    "\\begin{align*}\n",
    "j2 &= (1+j)^2 \\\\ j2&=1^2+2\\cdot 1\\cdot j +j^2 \\\\ j2&= 1+j2-1\\\\ j2&=j2\\\\\n",
    "\n",
    "z&= \\frac{[(1+j)^2]^40-[(1+j)^2]^41}{j^96} \\\\\n",
    "z &= \\frac{(j2)^40-(j2)^41}{j^0} = 2^40j^40-2^41j^41\\\\\n",
    "z&= 2^40(j^40 - 2j^41)=2^40(j^0-2j^1)\\\\ z&= 2^40(1-j2)\n",
    "\\end{align*}\n",
    "$$\n",
    "\n"
   ]
  },
  {
   "attachments": {},
   "cell_type": "markdown",
   "metadata": {},
   "source": [
    "$9.\\ Calcule as seguintes potências de j:\\\\$\n",
    "$a) j^76$\n",
    "$$\n",
    "\\begin{align*}\n",
    "j^76&=j^0=1\n",
    "\\end{align*}\n",
    "$$\n",
    "\n",
    "$b) j^110$\n",
    "$$\n",
    "\\begin{align*}\n",
    "j^110&=j^2=-1\n",
    "\\end{align*}\n",
    "$$ \n",
    "\n",
    "$c) j^97$\n",
    "$$\n",
    "\\begin{align*}\n",
    "j^97&=j^1=j\n",
    "\\end{align*}\n",
    "$$\n",
    "\n",
    "$d) j^97$\n",
    "$$\n",
    "\\begin{align*}\n",
    "j^503&=j^3=-j\n",
    "\\end{align*}\n",
    "$$"
   ]
  },
  {
   "attachments": {},
   "cell_type": "markdown",
   "metadata": {},
   "source": [
    "$10.\\ Prove\\ que\\ (1-j)^2\\ = -j2\\ e\\ calcule\\ (1-j)^96+(1+j)^97$\\\\\n",
    "$$\n",
    "\\begin{align*}\n",
    "-j2&=(1-j)^2\\\\-j2&= 1^2-2\\cdot 1j+j^2\\\\-j2&=1-j2-1\\\\-j2&=-j2\\\\ \\\\\n",
    "(1-j)^96+(1-j)^97 &= [(1-j)^2]^48+[(1-j)^2]^48\\cdot(1-j)\\\\\n",
    "(1-j)^96+(1-j)^97 &=(-j2)^48+(-j2)^48(1-j)\\\\\n",
    "(1-j)^96+(1-j)^97 &= (-2)^48j^48+(-2)^48j^48(1-j)\\\\\n",
    "(1-j)^96+(1-j)^97 &= (-2)^48j^0+(-2)^48j^0(1-j)\\\\\n",
    "(1-j)^96+(1-j)^97 &=(-2)^48+[(1-j)+1]\n",
    "\\end{align*}\n",
    "$$ "
   ]
  },
  {
   "attachments": {},
   "cell_type": "markdown",
   "metadata": {},
   "source": [
    "$11. Se\\ j^2=-1, calcule\\ o\\ valor\\ de\\ (1+j)^12-(1-j)^12.$\\\\\n",
    "$$\n",
    "\\begin{align*}\n",
    "(1+j)^12-(1-j)^12&= [(1+j)^2]^6-[(1-j)^2]^6\\\\&=(j2)^6-(-j2)^2\\\\\n",
    "&= j^62^6-(-2)^6j^6\\\\ &= j^6(2^6+2^6)\\\\ &= j^3j^3(64+64)\\\\ &=(-j)(-j)(128)\\\\ &=j^2128=-128\n",
    "\\end{align*}\n",
    "$$ "
   ]
  },
  {
   "attachments": {},
   "cell_type": "markdown",
   "metadata": {},
   "source": [
    "$12. Qual\\ o\\ resultado\\ da\\ simplificação \\ de:\\\\$\n",
    "$$\n",
    "\\begin{align*}\n",
    "\\frac{(2+j)^101\\cdot (2-j)^50}{(-2-j)^100\\cdot (j-2)^49}\\\\\n",
    "\\frac{(2+j)(2-j)(2+j)^100(2-j)^49}{(-2-j)(j-2)(-2-j)^99(j-2)^48}\\\\\n",
    "\\frac{5(2+j)^100(2-j)^49}{5(-2-j)^99(j-2^48)}\\\\\n",
    "\\frac{5^50(2+j)^51}{5^49(-2-j)^51}\\\\\n",
    "5(-1)^51=-5\n",
    "\\end{align*}\n",
    "$$ "
   ]
  },
  {
   "attachments": {},
   "cell_type": "markdown",
   "metadata": {},
   "source": [
    "$13. A\\ igualdade\\ (1+j)^n = (1-j)^n\\ verifica-se\\ para\\ os\\ números\\ naturais\\ divisiveis\\ por\\ qual\\ núnero\\ natural?$"
   ]
  },
  {
   "attachments": {},
   "cell_type": "markdown",
   "metadata": {},
   "source": [
    "14- Determine $x  \\in \\mathbb{R}\\ e\\ y\\ \\in \\mathbb{R}$ para que se tenha: \n",
    "\n",
    "$a)2+j3y=x+j9$\n",
    "$$\n",
    "\\begin{align*}\n",
    "\\begin{cases}\n",
    "x=2\\\\ 3y=9\n",
    "\\end{cases}\\\\ \n",
    "\\end{align*}\n",
    "$$ \n",
    "$S:(2,3)$\n",
    "\n",
    "$b)(x+jy)(3+j4)=7+j26\\\\ 3x+j4x+j3y+4yj^2=7+j26\\\\ 3x+j4x+j3y-4y$\n",
    "$$\n",
    "\\begin{align*}\n",
    "\\begin{cases}\n",
    "3x-4y=7\\\\ 4x+3y=26\\\\\n",
    "\\end{cases}\\\\ \n",
    "Multiplicando\\ a\\ primeira\\ equação\\ por\\ 3\\ a\\ segunda\\ por\\ 4\\ temos:\\\\\n",
    "\\begin{cases}\n",
    "9x-12y=21\\\\ 16x+12y =104\n",
    "\\end{cases}\\\\ \n",
    "somando\\ duas\\ equações\\ tempos\\:\\\\\n",
    "25x=125\\\\ x=5\\\\ portanto:\\\\ 3\\cdot x -4y=7\\\\\n",
    "y=\\frac{3\\cdot x -7}{4}=2\n",
    "\\end{align*}\n",
    "$$ \n",
    "$S:(5,2)\\\\ \\\\$\n",
    "\n",
    "$c) (x+jy)^2=j4\\\\ x^2+2xjy+(jy)^2=j4\\\\ x^2-y^2+j2xy=j4$\n",
    "$$\n",
    "\\begin{align*}\n",
    "\\begin{cases}\n",
    "x^2-y^2=0 \\\\ 2xy =4\\\\\n",
    "\\end{cases}\\\\ \n",
    "x=\\frac{2}{y}\\\\\n",
    "\\frac{4}{y^2}-y^2=0\\\\ y^4=4\\\\ y=4^\\frac{1}{4}\\\\\n",
    "x=\\frac{2}{y}=\\frac{2}{4^\\frac{1}{4}}\n",
    "\\end{align*}\n",
    "$$ \n",
    "$S:(\\frac{2}{4^\\frac{1}{4}},4^\\frac{1}{4})\\\\ \\\\$\n",
    "\n"
   ]
  },
  {
   "attachments": {},
   "cell_type": "markdown",
   "metadata": {},
   "source": [
    "15. Determine $x  \\in \\mathbb{R}\\ e\\ y\\ \\in \\mathbb{R}$ para que se tenha:\n",
    "\n",
    "$\\\\ a)\\ 3+j5x= y-j15$\n",
    "$$\n",
    "\\begin{align*}\n",
    "\\begin{cases}\n",
    "y=3\\\\ -5x=15\n",
    "\\end{cases}\\\\\n",
    "-5x=15\\\\ x=-3\n",
    "\\end{align*}\n",
    "$$ \n",
    "$S:(-3,3)\\\\$\n",
    "\n",
    "$b)(x+jy)(2+j3)= 1+j8\\\\ 2x+j3x+j2y+3yj^2=1+j8\\\\ 2x+j3x+j2y-3y=1+j8$\n",
    "$$\n",
    "\\begin{align*}\n",
    "\\begin{cases}\n",
    "2x-3y=1\\\\ 3x+2y=8\n",
    "\\end{cases}\\\\\n",
    "\\begin{cases}\n",
    "4x-6y=2\\\\ 9x+6y=24\n",
    "\\end{cases}\\\\\n",
    "13x=26\\\\ x=2\\\\ 2x-3y=1\\\\ y=1\n",
    "\\end{align*}\n",
    "$$ \n",
    "$S:(2,1)\\\\$\n",
    "\n",
    "$c) (3+jy)+(x-j2)= 7-j5\\\\ x+jy=4-j3$\n",
    "\n",
    "$$\n",
    "\\begin{align*}\n",
    "\\begin{cases}\n",
    "x=4\\\\ y=-3\n",
    "\\end{cases}\\\\\n",
    "\\end{align*}\n",
    "$$ \n",
    "$S:(4,-3)\\\\$\n",
    "\n",
    "$d) (x+jy)^2=j2\\\\ x^2+2jyx+(jy)^2=j2\\\\ $\n",
    "\n",
    "$$\n",
    "\\begin{align*}\n",
    "\\begin{cases}\n",
    "x^2-y^2=0\\\\ 2xy=1\\\\\n",
    "\\end{cases}\\\\\n",
    "x=\\frac{1}{2y}\\\\ \\frac{1}{4y^2}-y^2=0\\\\\n",
    "y= \\frac{1}{(4)^\\frac{1}{4}}\\\\ x =\\frac{(4)^\\frac{1}{4}}{2}\n",
    "\\end{align*}\n",
    "$$ \n",
    "$S:(\\frac{1}{4^\\frac{1}{4}},\\frac{(4)^\\frac{1}{4}}{2})\\\\$\n",
    "\n",
    "$e) (2-x+3y)+2yj=0\\\\ -x+3y+j2y=-2$\n",
    "$$\n",
    "\\begin{align*}\n",
    "\\begin{cases}\n",
    "-x+3y=-2 \\\\ 2y=0\n",
    "\\end{cases}\\\\\n",
    "y=0\\\\ -x+3\\cdot 0 =-2\\\\ x=2\n",
    "\\end{align*}\n",
    "$$ \n",
    "$S:(2,0)\\\\$\n",
    "\n",
    "$f) (3-j)(x+jy)=20\\\\ 3x+y+j3y-jx=20\\\\$\n",
    "\\begin{align*}\n",
    "\\begin{cases}\n",
    "3x+y=20\\\\ -x+3y=0\n",
    "\\end{cases}\\\\\n",
    "\\begin{cases}\n",
    "3x+y=20\\\\ -3x+9y=0\n",
    "\\end{cases}\\\\\n",
    "10y=20\\\\ y= 2\\\\ 3x+2=20\\\\x=6\n",
    "\\end{align*}\\\\\n",
    "$$ \n"
   ]
  },
  {
   "attachments": {},
   "cell_type": "markdown",
   "metadata": {},
   "source": [
    "16. Quais os números complexos $x\\ e\\ y$ para quais $x+jy=j\\ e\\ jx+y=j2-1\\\\$\n",
    "tomando $x\\ e\\ y$ como $a+jb$, temos:\n",
    "\n",
    "$$\n",
    "\\begin{align*}\n",
    "a+jb+j(a+jb)=j\\\\ a-b+jb+ja=j\\\\\n",
    "\\begin{cases}\n",
    "a-b=0\\\\ a+b=1\n",
    "\\end{cases}\n",
    "\\end{align*}\n",
    "2a=1\\\\ a=\\frac{1}{2}\\\\ b=\\frac{1}{2}\n",
    "$$ \n",
    "$S:(\\frac{1}{2},\\frac{1}{2})\\\\$\n",
    "\n",
    "$$\n",
    "\\begin{align*}\n",
    "j(a+jb)+a+jb=j2-1\\\\ a-b+ja+jb=j2-1\\\\\n",
    "\\begin{cases}\n",
    "a-b=-1\\\\ a+b=2\\\\\n",
    "\\end{cases}\n",
    "2a=1\\\\ a=\\frac{1}{2}\\\\ b=\\frac{3}{2}\n",
    "\\end{align*}\n",
    "\n",
    "$$ \n",
    "$S:(\\frac{1}{2},\\frac{3}{2})\\\\$\n"
   ]
  }
 ],
 "metadata": {
  "kernelspec": {
   "display_name": "Python 3",
   "language": "python",
   "name": "python3"
  },
  "language_info": {
   "codemirror_mode": {
    "name": "ipython",
    "version": 3
   },
   "file_extension": ".py",
   "mimetype": "text/x-python",
   "name": "python",
   "nbconvert_exporter": "python",
   "pygments_lexer": "ipython3",
   "version": "3.11.1"
  },
  "orig_nbformat": 4
 },
 "nbformat": 4,
 "nbformat_minor": 2
}
